src/proof/controllers/statefulset/pod.v
@@ -1,10 +1,12 @@
 From New.proof Require Import prelude empty_ffi.
+From New.proof.map Require Import for_range.
 From New.proof.string Require Export prefix_suffix.
 From New.proof.kubernetes_model Require Export get index create delete.
 From New.proof Require Export util.
 From New.proof Require Export wp_helpers.
 From New.proof.controllers Require Export common.
 From New.proof.controllers.statefulset Require Export ordinal.
+From New.proof.controllers.statefulset Require Export pvc.
 From New.proof.controllers.statefulset Require Export statefulset_init.
 From New.proof.k8s_io.api.apps Require Export v1.
 From New.proof.k8s_io.kubernetes.pkg Require Export controller.
@@ -163,18 +165,6 @@ Proof.
   - rewrite lookup_insert_eq. done.
 Qed.
 
-(* [ordinalOf] parses the decimal suffix following the last dash, without
-   checking that the preceding parent name belongs to the StatefulSet. *)
-Definition pod_ordinal_suffix (pod_name : go_string) : option go_string :=
-  match list_find (λ b, b = byte_dash) (reverse pod_name) with
-  | Some (idx, _) => Some (reverse (take idx (reverse pod_name)))
-  | None => None
-  end.
-
-Definition parse_pod_ordinal (pod_name : go_string) : option nat :=
-  suffix ← pod_ordinal_suffix pod_name;
-  parse_decimal_string suffix.
-
 (* Go map insertion overwrites an earlier volume with the same name, so the
    left fold preserves the last volume from the Pod's volume slice. *)
 Definition pod_volumes_map_insert
@@ -185,6 +175,226 @@ Definition pod_volumes_map_insert
 Definition pod_volumes_map_of_list (volumes : list VolumeV.t) :
     gmap go_string VolumeV.t :=
   fold_left pod_volumes_map_insert volumes ∅.
+
+Definition pod_physical_volumes_map_insert
+    (volumes : gmap go_string v1.Volume.t) (volume : v1.Volume.t) :
+    gmap go_string v1.Volume.t :=
+  <[volume.(v1.Volume.Name') := volume]> volumes.
+
+Definition pod_physical_volumes_map_of_list (volumes : list v1.Volume.t) :
+    gmap go_string v1.Volume.t :=
+  fold_left pod_physical_volumes_map_insert volumes ∅.
+
+Lemma pod_physical_volumes_map_of_list_snoc volumes volume :
+  pod_physical_volumes_map_of_list (volumes ++ [volume]) =
+    pod_physical_volumes_map_insert
+      (pod_physical_volumes_map_of_list volumes) volume.
+Proof.
+  unfold pod_physical_volumes_map_of_list. by rewrite fold_left_app.
+Qed.
+
+Definition volume_maps_related (R : v1.Volume.t → VolumeV.t → Prop)
+    (physical : gmap go_string v1.Volume.t)
+    (pure : gmap go_string VolumeV.t) : Prop :=
+  ∀ name physical_volume,
+    physical !! name = Some physical_volume →
+    ∃ pure_volume, pure !! name = Some pure_volume ∧
+      R physical_volume pure_volume.
+
+Lemma volume_maps_related_insert R physical pure physical_volume pure_volume :
+  physical_volume.(v1.Volume.Name') = pure_volume.(VolumeV.Name') →
+  R physical_volume pure_volume →
+  volume_maps_related R physical pure →
+  volume_maps_related R
+    (pod_physical_volumes_map_insert physical physical_volume)
+    (pod_volumes_map_insert pure pure_volume).
+Proof.
+  intros Hname HR Hrelated name volume Hlookup.
+  unfold pod_physical_volumes_map_insert in Hlookup.
+  unfold pod_volumes_map_insert.
+  apply lookup_insert_Some in Hlookup as
+    [[Hkey Hvolume]|[Hkey Hlookup]].
+  - subst name volume. exists pure_volume.
+    rewrite -Hname lookup_insert_eq. split; done.
+  - destruct (Hrelated _ _ Hlookup) as (pure_volume' & Hpure & HR').
+    exists pure_volume'. rewrite lookup_insert_ne.
+    + intros Heq. apply Hkey. rewrite Hname. exact Heq.
+    + split; done.
+Qed.
+
+Lemma volume_maps_related_fold R physical_volumes pure_volumes physical pure :
+  Forall2
+    (λ physical_volume pure_volume,
+      physical_volume.(v1.Volume.Name') = pure_volume.(VolumeV.Name') ∧
+      R physical_volume pure_volume)
+    physical_volumes pure_volumes →
+  volume_maps_related R physical pure →
+  volume_maps_related R
+    (fold_left pod_physical_volumes_map_insert physical_volumes physical)
+    (fold_left pod_volumes_map_insert pure_volumes pure).
+Proof.
+  intros Hvolumes. revert physical pure.
+  induction Hvolumes as [|physical_volume pure_volume physical_volumes
+      pure_volumes [Hname HR] Hvolumes IH]; intros physical pure Hrelated;
+    simpl; first done.
+  apply IH. by apply volume_maps_related_insert.
+Qed.
+
+Lemma Forall2_volume_names_with_lookup physical_volumes pure_volumes :
+  Forall2
+    (λ physical_volume pure_volume,
+      physical_volume.(v1.Volume.Name') = pure_volume.(VolumeV.Name'))
+    physical_volumes pure_volumes →
+  Forall2
+    (λ physical_volume pure_volume,
+      physical_volume.(v1.Volume.Name') = pure_volume.(VolumeV.Name') ∧
+      ∃ i, physical_volumes !! i = Some physical_volume ∧
+        pure_volumes !! i = Some pure_volume)
+    physical_volumes pure_volumes.
+Proof.
+  intros Hvolumes.
+  induction Hvolumes as [|physical_volume pure_volume physical_volumes
+      pure_volumes Hname Hvolumes IH]; constructor; first split.
+  - exact Hname.
+  - exists 0%nat. done.
+  - eapply Forall2_impl.
+    2: exact IH.
+    intros physical_volume' pure_volume'
+      (Hname' & i & Hphysical & Hpure).
+    split; first done. exists (S i). simpl. split; done.
+Qed.
+
+Lemma pod_volumes_maps_related physical_volumes pure_volumes :
+  Forall2
+    (λ physical_volume pure_volume,
+      physical_volume.(v1.Volume.Name') = pure_volume.(VolumeV.Name'))
+    physical_volumes pure_volumes →
+  volume_maps_related
+    (λ physical_volume pure_volume,
+      ∃ i, physical_volumes !! i = Some physical_volume ∧
+        pure_volumes !! i = Some pure_volume)
+    (pod_physical_volumes_map_of_list physical_volumes)
+    (pod_volumes_map_of_list pure_volumes).
+Proof.
+  intros Hvolumes.
+  apply volume_maps_related_fold.
+  - by apply Forall2_volume_names_with_lookup.
+  - intros name physical_volume Hlookup.
+    rewrite lookup_empty in Hlookup. done.
+Qed.
+
+Definition pure_volume_maps_related
+    (R : v1.Volume.t → VolumeV.t → Prop)
+    (pure : gmap go_string VolumeV.t)
+    (physical : gmap go_string v1.Volume.t) : Prop :=
+  ∀ name pure_volume,
+    pure !! name = Some pure_volume →
+    ∃ physical_volume, physical !! name = Some physical_volume ∧
+      R physical_volume pure_volume.
+
+Lemma pure_volume_maps_related_insert R physical pure physical_volume
+    pure_volume :
+  physical_volume.(v1.Volume.Name') = pure_volume.(VolumeV.Name') →
+  R physical_volume pure_volume →
+  pure_volume_maps_related R pure physical →
+  pure_volume_maps_related R
+    (pod_volumes_map_insert pure pure_volume)
+    (pod_physical_volumes_map_insert physical physical_volume).
+Proof.
+  intros Hname HR Hrelated name volume Hlookup.
+  unfold pod_volumes_map_insert in Hlookup.
+  unfold pod_physical_volumes_map_insert.
+  apply lookup_insert_Some in Hlookup as
+    [[Hkey Hvolume]|[Hkey Hlookup]].
+  - subst name volume. exists physical_volume.
+    rewrite Hname lookup_insert_eq. split; done.
+  - destruct (Hrelated _ _ Hlookup) as
+      (physical_volume' & Hphysical & HR').
+    exists physical_volume'. rewrite lookup_insert_ne.
+    + intros Heq. apply Hkey. rewrite -Hname. exact Heq.
+    + split; done.
+Qed.
+
+Lemma pure_volume_maps_related_fold R physical_volumes pure_volumes
+    physical pure :
+  Forall2
+    (λ physical_volume pure_volume,
+      physical_volume.(v1.Volume.Name') = pure_volume.(VolumeV.Name') ∧
+      R physical_volume pure_volume)
+    physical_volumes pure_volumes →
+  pure_volume_maps_related R pure physical →
+  pure_volume_maps_related R
+    (fold_left pod_volumes_map_insert pure_volumes pure)
+    (fold_left pod_physical_volumes_map_insert physical_volumes physical).
+Proof.
+  intros Hvolumes. revert physical pure.
+  induction Hvolumes as [|physical_volume pure_volume physical_volumes
+      pure_volumes [Hname HR] Hvolumes IH]; intros physical pure Hrelated;
+    simpl; first done.
+  apply IH. by apply pure_volume_maps_related_insert.
+Qed.
+
+Lemma pod_volumes_maps_reverse_related physical_volumes pure_volumes :
+  Forall2
+    (λ physical_volume pure_volume,
+      physical_volume.(v1.Volume.Name') = pure_volume.(VolumeV.Name'))
+    physical_volumes pure_volumes →
+  pure_volume_maps_related
+    (λ physical_volume pure_volume,
+      ∃ i, physical_volumes !! i = Some physical_volume ∧
+        pure_volumes !! i = Some pure_volume)
+    (pod_volumes_map_of_list pure_volumes)
+    (pod_physical_volumes_map_of_list physical_volumes).
+Proof.
+  intros Hvolumes. apply pure_volume_maps_related_fold.
+  - by apply Forall2_volume_names_with_lookup.
+  - intros name pure_volume Hlookup.
+    rewrite lookup_empty in Hlookup. done.
+Qed.
+
+Lemma objectmeta_deepown_name physical_meta pure_meta dq :
+  ObjectMetaV.deepown physical_meta pure_meta dq ⊢
+    ⌜ physical_meta.(v1.ObjectMeta.Name') = pure_meta.(ObjectMetaV.Name') ⌝ ∗
+    ObjectMetaV.deepown physical_meta pure_meta dq.
+Proof.
+  iIntros "Hmeta". iNamed "Hmeta".
+  iSplit; first done.
+  rewrite /ObjectMetaV.deepown. iFrame. iFrame "%".
+Qed.
+
+Lemma volume_deepown_name physical_volume pure_volume dq :
+  VolumeV.deepown physical_volume pure_volume dq ⊢
+    ⌜ physical_volume.(v1.Volume.Name') = pure_volume.(VolumeV.Name') ⌝ ∗
+    VolumeV.deepown physical_volume pure_volume dq.
+Proof.
+  iIntros "Hvolume". iNamed "Hvolume".
+  iSplit; first done. iFrame. iFrame "%".
+Qed.
+
+Lemma volume_deepown_list_names physical_volumes pure_volumes dq :
+  ([∗ list] physical_volume;pure_volume ∈ physical_volumes;pure_volumes,
+      VolumeV.deepown physical_volume pure_volume dq) ⊢
+    ⌜ Forall2
+        (λ physical_volume pure_volume,
+          physical_volume.(v1.Volume.Name') = pure_volume.(VolumeV.Name'))
+        physical_volumes pure_volumes ⌝ ∗
+    ([∗ list] physical_volume;pure_volume ∈ physical_volumes;pure_volumes,
+      VolumeV.deepown physical_volume pure_volume dq).
+Proof.
+  iInduction physical_volumes as [|physical_volume physical_volumes]
+    "IH" forall (pure_volumes).
+  - destruct pure_volumes; simpl.
+    + iIntros "H". iFrame. done.
+    + iIntros "%Hfalse". done.
+  - destruct pure_volumes as [|pure_volume pure_volumes]; simpl.
+    + iIntros "%Hfalse". done.
+    + iIntros "[Hvolume Hvolumes]".
+      iDestruct (volume_deepown_name with "Hvolume") as
+        "[%Hname Hvolume]".
+      iDestruct ("IH" with "Hvolumes") as "[%Hnames Hvolumes]".
+      iSplit; first by iPureIntro; constructor.
+      iFrame.
+Qed.
 
 Definition pod_volume_claim_matches
     (volumes : gmap go_string VolumeV.t) (set_name : go_string)
@@ -716,9 +926,7 @@ Lemma wp_storageMatches set_l pod_l (set : StatefulSetV.t) (pod : PodV.t)
     dq_set dq_pod :
   {{{ "Hset" ∷ StatefulSetV.deepown_l set_l set dq_set ∗
       "Hpod" ∷ PodV.deepown_l pod_l pod dq_pod ∗
-      "%Hpod_name_len" ∷
-        ⌜ Z.of_nat (length pod.(PodV.ObjectMeta').(ObjectMetaV.Name')) <=
-          go_int_max ⌝
+      "%Hpod_name_len" ∷ ⌜ Z.of_nat (length pod.(PodV.ObjectMeta').(ObjectMetaV.Name')) <= go_int_max ⌝
   }}}
     @! statefulset.storageMatches #set_l #pod_l
   {{{ (ret : bool), RET #ret;
@@ -726,7 +934,515 @@ Lemma wp_storageMatches set_l pod_l (set : StatefulSetV.t) (pod : PodV.t)
       "Hpod" ∷ PodV.deepown_l pod_l pod dq_pod ∗
       "%Hret" ∷ ⌜ ret = true ↔ pod_storage_matches set pod ⌝
   }}}.
-Proof. Admitted.
+Proof.
+  wp_start as "H". iNamed "H".
+  iPoseProof (PodV.deepown_l_split with "Hpod") as
+    "(%Hpod_l_not_null & Hpod_typemeta & Hpod_objectmeta_l & Hpod_spec_l & Hpod_status_l)".
+  iDestruct "Hpod_objectmeta_l" as (pod_meta_c)
+    "[Hpod_objectmeta_field Hpod_objectmeta]".
+  iNamedPrefix "Hpod_objectmeta" "Hpod_meta_".
+  iDestruct "Hpod_spec_l" as (pod_spec_c)
+    "[Hpod_spec_field Hpod_spec]".
+  iNamedPrefix "Hpod_spec" "Hpod_spec_".
+  iDestruct "Hpod_spec_Hdeepown_volumes" as (physical_volumes)
+    "Hpod_volumes".
+  rewrite /deepown_list.
+  iDestruct "Hpod_volumes" as
+    "[Hpod_volumes_slice Hpod_volumes_deepown]".
+  iDestruct (own_slice_len with "Hpod_volumes_slice") as
+    %(Hpod_volumes_len1 & Hpod_volumes_len2).
+  iDestruct (own_slice_wf with "Hpod_volumes_slice") as
+    %Hpod_volumes_cap.
+  iDestruct (big_sepL2_length with "Hpod_volumes_deepown") as
+    %Hpod_volumes_deepown_len.
+  Ltac restore_storage_pod pod_spec_c physical_volumes pod_meta_c pod
+      dq_pod pod_l Hpod_l_not_null :=
+    iAssert (∃ volumes,
+        deepown_list pod_spec_c.(v1.PodSpec.Volumes') volumes
+          pod.(PodV.Spec').(PodSpecV.Volumes')
+          (λ physical_volume pure_volume,
+            VolumeV.deepown physical_volume pure_volume dq_pod))%I
+      with "[Hpod_volumes_slice Hpod_volumes_deepown]" as
+        "Hpod_spec_Hdeepown_volumes";
+    [ iExists physical_volumes; rewrite /deepown_list; iFrame | ];
+    iCombineNamed "Hpod_meta_*" as "Hpod_objectmeta";
+    iAssert (ObjectMetaV.deepown pod_meta_c
+        pod.(PodV.ObjectMeta') dq_pod)
+      with "[Hpod_objectmeta]" as "Hpod_objectmeta";
+    [ iNamed "Hpod_objectmeta"; iFrame; done | ];
+    iAssert (ObjectMetaV.deepown_l (PodV.objectmeta_ptr pod_l)
+        pod.(PodV.ObjectMeta') dq_pod)
+      with "[Hpod_objectmeta_field Hpod_objectmeta]" as
+        "Hpod_objectmeta_l";
+    [ iExists pod_meta_c; iFrame | ];
+    iCombineNamed "Hpod_spec_H*" as "Hpod_spec";
+    iAssert (PodSpecV.deepown pod_spec_c pod.(PodV.Spec') dq_pod)
+      with "[Hpod_spec]" as "Hpod_spec";
+    [ iNamed "Hpod_spec"; iFrame; done | ];
+    iAssert (PodSpecV.deepown_l (PodV.spec_ptr pod_l)
+        pod.(PodV.Spec') dq_pod)
+      with "[Hpod_spec_field Hpod_spec]" as "Hpod_spec_l";
+    [ iExists pod_spec_c; iFrame | ];
+    iPoseProof (PodV.deepown_l_restore _ _ _ Hpod_l_not_null
+      with "[$Hpod_typemeta $Hpod_objectmeta_l $Hpod_spec_l $Hpod_status_l]")
+      as "Hpod".
+  wp_auto.
+  wp_apply (wp_ordinalOf_parse (v1.ObjectMeta.Name' pod_meta_c) with "[]").
+  { iPureIntro. rewrite Hpod_meta_Hdeepown_name. exact Hpod_name_len. }
+  iIntros (ordinal) "%Hordinal".
+  rewrite Hpod_meta_Hdeepown_name in Hordinal.
+  wp_auto.
+  destruct (parse_pod_ordinal
+      pod.(PodV.ObjectMeta').(ObjectMetaV.Name')) as [expected_ordinal|]
+    eqn:Hparse_ordinal.
+  2: {
+    simpl in Hordinal.
+    wp_if_destruct.
+    2: { exfalso. word. }
+    restore_storage_pod pod_spec_c physical_volumes pod_meta_c pod
+      dq_pod pod_l Hpod_l_not_null.
+    iApply ("HΦ" $! false). iFrame. iPureIntro.
+    split; first done. intros Hmatches.
+    unfold pod_storage_matches in Hmatches.
+    by rewrite Hparse_ordinal in Hmatches.
+  }
+  destruct (decide (expected_ordinal <= go_int32_max_nat)%nat) as
+    [Hordinal_bound|Hordinal_overflow].
+  2: {
+    simpl in Hordinal.
+    wp_if_destruct.
+    2: { exfalso. word. }
+    restore_storage_pod pod_spec_c physical_volumes pod_meta_c pod
+      dq_pod pod_l Hpod_l_not_null.
+    iApply ("HΦ" $! false). iFrame. iPureIntro.
+    split; first done. intros Hmatches.
+    unfold pod_storage_matches in Hmatches.
+    rewrite Hparse_ordinal in Hmatches. destruct Hmatches. done.
+  }
+  simpl in Hordinal.
+  wp_if_destruct.
+  { exfalso. word. }
+  wp_apply wp_map_make2 as "%volumes_map Hvolumes_map".
+  set I := (∃ (i : w64) (volume : v1.Volume.t) (volumes_l : map.t),
+    "Hi_ptr" ∷ i_ptr ↦ i ∗
+    "Hvolume_ptr" ∷ volume_ptr ↦ volume ∗
+    "Hvolumes_ptr" ∷ volumes_ptr ↦ volumes_l ∗
+    "Hpod_volumes_slice" ∷
+      pod_spec_c.(v1.PodSpec.Volumes') ↦* physical_volumes ∗
+    "Hvolumes_map" ∷ volumes_l ↦$
+      pod_physical_volumes_map_of_list
+        (take (sint.nat i) physical_volumes) ∗
+    "%Hi" ∷ ⌜ 0 ≤ sint.Z i ≤
+      sint.Z (slice.len pod_spec_c.(v1.PodSpec.Volumes')) ⌝
+  )%I.
+  iAssert I with "[i volume volumes Hpod_volumes_slice Hvolumes_map]"
+    as "Hloop_inv".
+  { iExists (W64 0), (zero_val v1.Volume.t), volumes_map.
+    rewrite take_0 /pod_physical_volumes_map_of_list /=.
+    iFrame. iPureIntro. word. }
+  wp_for "Hloop_inv". wp_if_destruct.
+  - destruct (decide (0 ≤ sint.Z i <
+      sint.Z (slice.len pod_spec_c.(v1.PodSpec.Volumes')))) as
+      [_|Hbounds]; last word.
+    assert (∃ this_volume,
+      physical_volumes !! sint.nat i = Some this_volume) as
+      [this_volume Hthis_volume_lookup].
+    { apply lookup_lt_is_Some_2. rewrite Hpod_volumes_len1. word. }
+    wp_apply (wp_load_slice_index with "[$Hpod_volumes_slice]");
+      [word| |].
+    { iPureIntro. exact Hthis_volume_lookup. }
+    iIntros "Hpod_volumes_slice". wp_auto.
+    wp_apply (wp_map_insert go.string with "[$Hvolumes_map]").
+    iIntros "Hvolumes_map". wp_auto.
+    iApply wp_for_post_do. wp_auto. iFrame "HΦ".
+    iFrame "Hset Hpod_typemeta Hpod_objectmeta_field Hpod_spec_field
+      Hpod_status_l Hpod_volumes_deepown".
+    iFrame.
+    assert (pod_physical_volumes_map_of_list
+      (take (sint.nat (word.add i (W64 1))) physical_volumes) =
+      pod_physical_volumes_map_insert
+        (pod_physical_volumes_map_of_list
+          (take (sint.nat i) physical_volumes)) this_volume) as Hmap_next.
+    { assert (sint.nat (word.add i (W64 1)) = S (sint.nat i)) as ->
+        by word.
+      rewrite (take_S_r _ _ _ Hthis_volume_lookup).
+      apply pod_physical_volumes_map_of_list_snoc. }
+    rewrite Hmap_next. iFrame. iFrame "%". iPureIntro. word.
+  - assert (take (sint.nat i) physical_volumes = physical_volumes)
+      as Htake_all.
+    { assert (sint.nat i = length physical_volumes) as Hi_len.
+      { rewrite Hpod_volumes_len1. word. }
+      rewrite Hi_len. apply take_ge. lia. }
+    rewrite Htake_all.
+    iDestruct (volume_deepown_list_names with
+      "Hpod_volumes_deepown") as
+      "[%Hvolume_names Hpod_volumes_deepown]".
+    pose proof (pod_volumes_maps_related _ _ Hvolume_names) as
+      Hvolumes_related.
+    pose proof (pod_volumes_maps_reverse_related _ _ Hvolume_names) as
+      Hvolumes_reverse_related.
+    wp_apply (wp_volumeClaimTemplatesByName set_l set dq_set with "Hset").
+    iIntros (set_phy claim_templates_map claim_templates_list
+      claim_templates_phy) "Hclaim_result".
+    iDestruct "Hclaim_result" as "(Hset_ptr & Hclaim_result)".
+    iNamed "Hclaim_result".
+    iAssert (StatefulSetV.deepown_l set_l set dq_set)
+      with "[Hset_ptr Hdeepown_objectmeta Hdeepown_replicas_some
+        Hdeepown_template Hdeepown_volumeclaimtemplates Hdeepown_status]"
+      as "Hset".
+    { iExists set_phy. rewrite /StatefulSetV.deepown.
+      iFrame. rewrite /StatefulSetSpecV.deepown.
+      iFrame. iFrame "%". }
+    iPoseProof (StatefulSetV.deepown_l_split with "Hset") as
+      "(%Hset_l_not_null & Hset_typemeta & Hset_objectmeta_l & Hset_spec_l & Hset_status_l)".
+    iDestruct "Hset_objectmeta_l" as (set_meta_c)
+      "[Hset_objectmeta_field Hset_objectmeta]".
+    iCombineNamed "Hpod_meta_*" as "Hpod_objectmeta".
+    iAssert (ObjectMetaV.deepown pod_meta_c pod.(PodV.ObjectMeta') dq_pod)
+      with "[Hpod_objectmeta]" as "Hpod_objectmeta".
+    { iNamed "Hpod_objectmeta". iFrame. done. }
+    iAssert (ObjectMetaV.deepown_l (PodV.objectmeta_ptr pod_l)
+        pod.(PodV.ObjectMeta') dq_pod)
+      with "[Hpod_objectmeta_field Hpod_objectmeta]" as
+        "Hpod_objectmeta_l".
+    { iExists pod_meta_c. iFrame. }
+    wp_auto.
+    set Q := (λ (last_claim : v1.PersistentVolumeClaim.t)
+        (last_name : go_string),
+      "Hset_typemeta" ∷
+        StatefulSetV.typemeta_ptr set_l ↦{dq_set} set.(StatefulSetV.TypeMeta') ∗
+      "Hset_objectmeta_field" ∷
+        StatefulSetV.objectmeta_ptr set_l ↦{dq_set} set_meta_c ∗
+      "Hset_objectmeta" ∷ ObjectMetaV.deepown set_meta_c
+        set.(StatefulSetV.ObjectMeta') dq_set ∗
+      "Hset_spec_l" ∷ StatefulSetSpecV.deepown_l
+        (StatefulSetV.spec_ptr set_l) set.(StatefulSetV.Spec') dq_set ∗
+      "Hset_status_l" ∷ StatefulSetStatusV.deepown_l
+        (StatefulSetV.status_ptr set_l) set.(StatefulSetV.Status') dq_set ∗
+      "Hpod_typemeta" ∷
+        PodV.typemeta_ptr pod_l ↦{dq_pod} pod.(PodV.TypeMeta') ∗
+      "Hpod_objectmeta_l" ∷ ObjectMetaV.deepown_l
+        (PodV.objectmeta_ptr pod_l) pod.(PodV.ObjectMeta') dq_pod ∗
+      "Hpod_spec_field" ∷ PodV.spec_ptr pod_l ↦{dq_pod} pod_spec_c ∗
+      "Hpod_volumes_slice" ∷
+        pod_spec_c.(v1.PodSpec.Volumes') ↦* physical_volumes ∗
+      "Hpod_volumes_deepown" ∷
+        ([∗ list] physical_volume;pure_volume ∈
+          physical_volumes;pod.(PodV.Spec').(PodSpecV.Volumes'),
+          VolumeV.deepown physical_volume pure_volume dq_pod) ∗
+      "Hpod_spec_rest" ∷
+        (⌜ pod_spec_c.(v1.PodSpec.Hostname') =
+          pod.(PodV.Spec').(PodSpecV.Hostname') ⌝ ∗
+         ⌜ pod_spec_c.(v1.PodSpec.Subdomain') =
+          pod.(PodV.Spec').(PodSpecV.Subdomain') ⌝) ∗
+      "Hpod_status_l" ∷ PodStatusV.deepown_l
+        (PodV.status_ptr pod_l) pod.(PodV.Status') dq_pod ∗
+      "Hvolumes_map" ∷ volumes_l ↦$
+        pod_physical_volumes_map_of_list physical_volumes ∗
+      "set" ∷ set_ptr ↦ set_l ∗
+      "ordinal" ∷ ordinal_ptr ↦ ordinal ∗
+      "volumes" ∷ volumes_ptr ↦ volumes_l ∗
+      "claim" ∷ claim_ptr ↦ last_claim ∗
+      "name" ∷ name_ptr ↦ last_name
+    )%I.
+    set P := (λ (keys : list go_string) (z : Z),
+      ∃ (last_claim : v1.PersistentVolumeClaim.t)
+        (last_name : go_string),
+      Q last_claim last_name ∗
+      "%Hprocessed" ∷ ⌜ ∀ claim_template_name,
+        claim_template_name ∈ take (Z.to_nat z) keys →
+        pod_volume_claim_matches
+          (pod_volumes_map_of_list
+            pod.(PodV.Spec').(PodSpecV.Volumes'))
+          set.(StatefulSetV.ObjectMeta').(ObjectMetaV.Name')
+          expected_ordinal claim_template_name ⌝
+    )%I.
+    set R := (λ bv,
+      ∃ (last_claim : v1.PersistentVolumeClaim.t)
+        (last_name : go_string),
+      Q last_claim last_name ∗
+      ⌜ bv = return_val #false ∧ ¬ pod_storage_matches set pod ⌝)%I.
+    wp_apply (wp_map_for_range_return_or_return
+      (key_type:=go.string) P R with "Hclaim_templates_map").
+    iIntros (keys) "%Hkeys".
+    iSplitL "Hset_typemeta Hset_objectmeta_field Hset_objectmeta
+      Hset_spec_l Hset_status_l Hpod_typemeta Hpod_objectmeta_l
+      Hpod_spec_field Hpod_volumes_slice Hpod_volumes_deepown
+      Hpod_status_l Hvolumes_map set ordinal Hvolumes_ptr claim name".
+    { iExists (zero_val v1.PersistentVolumeClaim.t), ""%go.
+      iFrame. iFrame "%".
+      iPureIntro. intros claim_template_name Hin.
+      rewrite take_0 in Hin. inversion Hin. }
+    iSplitL "".
+    { iModIntro. iIntros (z claim_template_name claim_template_phy)
+        "%Hiter HP".
+      destruct Hiter as (Hz_bounds & Hkey_lookup & Hclaim_lookup).
+      iDestruct "HP" as (last_claim last_name) "[HQ %Hprocessed]".
+      iNamed "HQ".
+      assert (claim_template_name ∈ pvc_claim_template_names set)
+        as Hclaim_name_in.
+      { assert (claim_template_name ∈ dom claim_templates_phy) as Hin_dom.
+        { apply elem_of_dom. eexists. exact Hclaim_lookup. }
+        rewrite Hclaim_templates_map_dom elem_of_list_to_set in Hin_dom.
+        exact Hin_dom. }
+      wp_auto. wp_alloc this_volume_ptr as "Hthis_volume_ptr".
+      wp_pures. wp_auto.
+      wp_apply (wp_map_lookup2 go.string v1.Volume volumes_l
+        (pod_physical_volumes_map_of_list physical_volumes)
+        claim_template_name (DfracOwn 1) with "[$Hvolumes_map]").
+      iIntros "Hvolumes_map".
+      destruct (pod_physical_volumes_map_of_list physical_volumes !!
+        claim_template_name) as [physical_volume|] eqn:Hphysical_lookup.
+      2: {
+        wp_auto.
+        iRight. iRight. iExists #false. iSplit; first done.
+        iExists claim_template_phy, claim_template_name. iFrame.
+        iPureIntro. split; first done.
+        unfold pod_storage_matches. rewrite Hparse_ordinal /=.
+        intros (_ & Hmatches).
+        rewrite Forall_forall in Hmatches.
+        specialize (Hmatches claim_template_name).
+        rewrite <- list_elem_of_In in Hmatches.
+        specialize (Hmatches Hclaim_name_in).
+        unfold pod_volume_claim_matches in Hmatches.
+        destruct (pod_volumes_map_of_list
+            pod.(PodV.Spec').(PodSpecV.Volumes') !! claim_template_name)
+          as [pure_volume|] eqn:Hpure_lookup; [|done].
+        destruct (Hvolumes_reverse_related _ _ Hpure_lookup) as
+          (physical_volume' & Hphysical_lookup' & _).
+        rewrite Hphysical_lookup in Hphysical_lookup'. done.
+      }
+      destruct (Hvolumes_related _ _ Hphysical_lookup) as
+        (pure_volume & Hpure_lookup & volume_index &
+          Hphysical_volume_index & Hpure_volume_index).
+      iDestruct (big_sepL2_lookup_acc with
+        "Hpod_volumes_deepown") as
+        "[Hcurrent_volume Hvolumes_restore]";
+        [exact Hphysical_volume_index|exact Hpure_volume_index|].
+      iDestruct "Hcurrent_volume" as
+        "(%Hcurrent_volume_name & Hcurrent_source)".
+      iDestruct "Hcurrent_source" as
+        "(%Hcurrent_pvc_none & Hcurrent_pvc_some)".
+      destruct pure_volume.(VolumeV.VolumeSource').(VolumeSourceV.PersistentVolumeClaim')
+        as [pure_pvc|] eqn:Hpure_pvc.
+      2: {
+        assert (physical_volume.(v1.Volume.VolumeSource').(v1.VolumeSource.PersistentVolumeClaim') =
+          null) as Hphysical_pvc_null.
+        { apply Hcurrent_pvc_none. done. }
+        assert (bool_decide
+            (physical_volume.(v1.Volume.VolumeSource').(v1.VolumeSource.PersistentVolumeClaim') =
+              null) = true) as Hphysical_pvc_null_bool.
+        { by apply bool_decide_eq_true_2. }
+        wp_auto.
+        rewrite Hphysical_pvc_null_bool.
+        wp_auto.
+        iAssert (VolumeV.deepown physical_volume pure_volume dq_pod)
+          with "[Hcurrent_pvc_some]" as "Hcurrent_volume".
+        { rewrite /VolumeV.deepown /VolumeSourceV.deepown Hpure_pvc.
+          iFrame. iFrame "%". }
+        iSpecialize ("Hvolumes_restore" with "Hcurrent_volume").
+        iRename "Hvolumes_restore" into "Hpod_volumes_deepown".
+        iRight. iRight. iExists #false. iSplit; first done.
+        iExists claim_template_phy, claim_template_name. iFrame.
+        iPureIntro. split; first done.
+        unfold pod_storage_matches. rewrite Hparse_ordinal /=.
+        intros (_ & Hmatches).
+        rewrite Forall_forall in Hmatches.
+        specialize (Hmatches claim_template_name).
+        rewrite <- list_elem_of_In in Hmatches.
+        specialize (Hmatches Hclaim_name_in).
+        unfold pod_volume_claim_matches in Hmatches.
+        rewrite Hpure_lookup Hpure_pvc in Hmatches. done.
+      }
+      iDestruct "Hcurrent_pvc_some" as (physical_pvc)
+        "[Hphysical_pvc %Hphysical_pvc]".
+      subst physical_pvc.
+      assert (physical_volume.(v1.Volume.VolumeSource').(v1.VolumeSource.PersistentVolumeClaim') ≠
+          null) as Hphysical_pvc_not_null.
+      { intros Hnull. apply Hcurrent_pvc_none in Hnull. done. }
+      assert (bool_decide
+          (physical_volume.(v1.Volume.VolumeSource').(v1.VolumeSource.PersistentVolumeClaim') =
+            null) = false) as Hphysical_pvc_not_null_bool.
+      { by apply bool_decide_eq_false_2. }
+      iDestruct (objectmeta_deepown_name with "Hset_objectmeta") as
+        "[%Hset_name Hset_objectmeta]".
+      iNamedPrefix "Hset_objectmeta" "Hset_meta_".
+      pose proof (Hclaim_templates_map_values _ _ Hclaim_lookup) as
+        [_ Hclaim_name].
+      wp_auto.
+      rewrite Hphysical_pvc_not_null_bool.
+      wp_auto.
+      wp_apply (wp_claimName
+        (v1.ObjectMeta.Name' set_meta_c)
+        (v1.ObjectMeta.Name'
+          claim_template_phy.(v1.PersistentVolumeClaim.ObjectMeta'))
+        ordinal with "[]").
+      { iPureIntro. word. }
+      assert (Hordinal_nat : sint.nat ordinal = expected_ordinal) by word.
+      assert (Hdesired_name :
+        v1.ObjectMeta.Name'
+            claim_template_phy.(v1.PersistentVolumeClaim.ObjectMeta') ++
+          "-"%go ++ v1.ObjectMeta.Name' set_meta_c ++ "-"%go ++
+          decimal_string (sint.nat ordinal) =
+        desired_pvc_name
+          set.(StatefulSetV.ObjectMeta').(ObjectMetaV.Name')
+          claim_template_name expected_ordinal).
+      { unfold desired_pvc_name.
+        rewrite Hclaim_name Hset_name Hordinal_nat. done. }
+      iCombineNamed "Hset_meta_*" as "Hset_objectmeta".
+      iAssert (ObjectMetaV.deepown set_meta_c
+          set.(StatefulSetV.ObjectMeta') dq_set)
+        with "[Hset_objectmeta]" as "Hset_objectmeta".
+      { iNamed "Hset_objectmeta". iFrame. done. }
+      wp_if_destruct.
+      - assert (Hcurrent_matches :
+          pod_volume_claim_matches
+            (pod_volumes_map_of_list
+              pod.(PodV.Spec').(PodSpecV.Volumes'))
+            set.(StatefulSetV.ObjectMeta').(ObjectMetaV.Name')
+            (sint.nat ordinal)
+            (v1.ObjectMeta.Name'
+              claim_template_phy.(v1.PersistentVolumeClaim.ObjectMeta'))).
+        { unfold pod_volume_claim_matches.
+          rewrite Hpure_lookup Hpure_pvc /=.
+          match goal with
+          | Heq : pure_pvc.(v1.PersistentVolumeClaimVolumeSource.ClaimName') = _ |- _ =>
+              rewrite -Hdesired_name; exact Heq
+          end. }
+        iAssert (∃ physical_pvc,
+          physical_volume.(v1.Volume.VolumeSource').(v1.VolumeSource.PersistentVolumeClaim')
+            ↦{dq_pod} physical_pvc ∗ ⌜ physical_pvc = pure_pvc ⌝)%I
+          with "[Hphysical_pvc]" as "Hcurrent_pvc_some".
+        { iExists pure_pvc. iFrame. done. }
+        iAssert (VolumeV.deepown physical_volume pure_volume dq_pod)
+          with "[Hcurrent_pvc_some]" as "Hcurrent_volume".
+        { rewrite /VolumeV.deepown /VolumeSourceV.deepown Hpure_pvc.
+          iFrame. iFrame "%". }
+        iSpecialize ("Hvolumes_restore" with "Hcurrent_volume").
+        iRename "Hvolumes_restore" into "Hpod_volumes_deepown".
+        iRight. iLeft. iSplit; first done.
+        iExists claim_template_phy,
+          (v1.ObjectMeta.Name'
+            claim_template_phy.(v1.PersistentVolumeClaim.ObjectMeta')).
+        iFrame.
+        iPureIntro. intros name' Hin.
+        replace (Z.to_nat (z + 1)) with (S (Z.to_nat z)) in Hin by lia.
+        rewrite (take_S_r _ _ _ Hkey_lookup) in Hin.
+        apply elem_of_app in Hin as [Hin|Hin].
+        + by apply Hprocessed.
+        + rewrite list_elem_of_singleton in Hin. subst name'.
+          exact Hcurrent_matches.
+      - iAssert (∃ physical_pvc,
+          physical_volume.(v1.Volume.VolumeSource').(v1.VolumeSource.PersistentVolumeClaim')
+            ↦{dq_pod} physical_pvc ∗ ⌜ physical_pvc = pure_pvc ⌝)%I
+          with "[Hphysical_pvc]" as "Hcurrent_pvc_some".
+        { iExists pure_pvc. iFrame. done. }
+        iAssert (VolumeV.deepown physical_volume pure_volume dq_pod)
+          with "[Hcurrent_pvc_some]" as "Hcurrent_volume".
+        { rewrite /VolumeV.deepown /VolumeSourceV.deepown Hpure_pvc.
+          iFrame. iFrame "%". }
+        iSpecialize ("Hvolumes_restore" with "Hcurrent_volume").
+        iRename "Hvolumes_restore" into "Hpod_volumes_deepown".
+        iRight. iRight. iExists #false. iSplit; first done.
+        iExists claim_template_phy,
+          (v1.ObjectMeta.Name'
+            claim_template_phy.(v1.PersistentVolumeClaim.ObjectMeta')).
+        iFrame.
+        iPureIntro. split; first done.
+        unfold pod_storage_matches. rewrite Hparse_ordinal /=.
+        intros (_ & Hmatches).
+        rewrite Forall_forall in Hmatches.
+        specialize (Hmatches
+          (v1.ObjectMeta.Name'
+            claim_template_phy.(v1.PersistentVolumeClaim.ObjectMeta'))).
+        rewrite <- list_elem_of_In in Hmatches.
+        specialize (Hmatches Hclaim_name_in).
+        unfold pod_volume_claim_matches in Hmatches.
+        rewrite Hpure_lookup Hpure_pvc in Hmatches. simpl in Hmatches.
+        match goal with
+        | Hneq : pure_pvc.(v1.PersistentVolumeClaimVolumeSource.ClaimName') ≠ _ |- _ =>
+            apply Hneq; rewrite Hdesired_name; exact Hmatches
+        end.
+    }
+    iIntros (bv) "Hclaim_templates_map Hresult".
+    iDestruct "Hresult" as "[Hdone|Hreturn]".
+    { iDestruct "Hdone" as "(%Hbv & Hdone)". subst bv.
+      iDestruct "Hdone" as (last_claim last_name)
+        "[HQ %Hprocessed]".
+      iNamed "HQ".
+      assert (Hstorage : pod_storage_matches set pod).
+      { unfold pod_storage_matches. rewrite Hparse_ordinal /=.
+        split; first exact Hordinal_bound.
+        rewrite Forall_forall. intros claim_template_name Hclaim_name.
+        apply Hprocessed.
+        destruct Hkeys as (Hkeys_dom & Hkeys_len & Hkeys_nodup).
+        assert (claim_template_name ∈
+            list_to_set (C:=gset go_string) keys) as Hclaim_key_set.
+        { rewrite -list_elem_of_In in Hclaim_name.
+          rewrite Hkeys_dom Hclaim_templates_map_dom elem_of_list_to_set.
+          exact Hclaim_name. }
+        apply elem_of_list_to_set in Hclaim_key_set as Hclaim_key.
+        replace (take (Z.to_nat (size claim_templates_phy)) keys) with keys.
+        - exact Hclaim_key.
+        - symmetry. apply take_ge. rewrite Nat2Z.id. lia. }
+      wp_auto.
+      iAssert (ObjectMetaV.deepown_l
+          (StatefulSetV.objectmeta_ptr set_l)
+          set.(StatefulSetV.ObjectMeta') dq_set)
+        with "[Hset_objectmeta_field Hset_objectmeta]" as
+          "Hset_objectmeta_l".
+      { iExists set_meta_c. iFrame. }
+      iPoseProof (StatefulSetV.deepown_l_restore _ _ _ Hset_l_not_null
+        with "[$Hset_typemeta $Hset_objectmeta_l $Hset_spec_l $Hset_status_l]")
+        as "Hset".
+      iDestruct "Hpod_spec_rest" as "(%Hpod_hostname & %Hpod_subdomain)".
+      iAssert (PodSpecV.deepown pod_spec_c pod.(PodV.Spec') dq_pod)
+        with "[Hpod_volumes_slice Hpod_volumes_deepown]" as "Hpod_spec".
+      { rewrite /PodSpecV.deepown.
+        iSplitL "Hpod_volumes_slice Hpod_volumes_deepown".
+        { iExists physical_volumes. rewrite /deepown_list. iFrame. }
+        iFrame "%". }
+      iAssert (PodSpecV.deepown_l (PodV.spec_ptr pod_l)
+          pod.(PodV.Spec') dq_pod)
+        with "[Hpod_spec_field Hpod_spec]" as "Hpod_spec_l".
+      { iExists pod_spec_c. iFrame. }
+      iPoseProof (PodV.deepown_l_restore _ _ _ Hpod_l_not_null
+        with "[$Hpod_typemeta $Hpod_objectmeta_l $Hpod_spec_l $Hpod_status_l]")
+        as "Hpod".
+      iApply ("HΦ" $! true). iFrame.
+      iPureIntro. split; [intros _; exact Hstorage|done]. }
+    { iDestruct "Hreturn" as (last_claim last_name)
+        "[HQ %Hreturn]".
+      destruct Hreturn as (Hbv & Hnot_storage). subst bv.
+      iNamed "HQ".
+      wp_auto.
+      iAssert (ObjectMetaV.deepown_l
+          (StatefulSetV.objectmeta_ptr set_l)
+          set.(StatefulSetV.ObjectMeta') dq_set)
+        with "[Hset_objectmeta_field Hset_objectmeta]" as
+          "Hset_objectmeta_l".
+      { iExists set_meta_c. iFrame. }
+      iPoseProof (StatefulSetV.deepown_l_restore _ _ _ Hset_l_not_null
+        with "[$Hset_typemeta $Hset_objectmeta_l $Hset_spec_l $Hset_status_l]")
+        as "Hset".
+      iDestruct "Hpod_spec_rest" as "(%Hpod_hostname & %Hpod_subdomain)".
+      iAssert (PodSpecV.deepown pod_spec_c pod.(PodV.Spec') dq_pod)
+        with "[Hpod_volumes_slice Hpod_volumes_deepown]" as "Hpod_spec".
+      { rewrite /PodSpecV.deepown.
+        iSplitL "Hpod_volumes_slice Hpod_volumes_deepown".
+        { iExists physical_volumes. rewrite /deepown_list. iFrame. }
+        iFrame "%". }
+      iAssert (PodSpecV.deepown_l (PodV.spec_ptr pod_l)
+          pod.(PodV.Spec') dq_pod)
+        with "[Hpod_spec_field Hpod_spec]" as "Hpod_spec_l".
+      { iExists pod_spec_c. iFrame. }
+      iPoseProof (PodV.deepown_l_restore _ _ _ Hpod_l_not_null
+        with "[$Hpod_typemeta $Hpod_objectmeta_l $Hpod_spec_l $Hpod_status_l]")
+        as "Hpod".
+      iApply ("HΦ" $! false). iFrame.
+      iPureIntro. split; [done|intros Hstorage; contradiction]. }
+  Unshelve. all: apply _.
+Qed.
 
 (* The ordinal and name preconditions exclude the failure result (-1) from
    ordinalOf. The helper mutates the Pod in place, so it requires full Pod
